src/program_proof/mvcc/tuple_read_version.v
@@ -194,17 +194,14 @@ Definition tuple_read tuple tid key val found γ : iProp Σ :=
     "%Htid" ∷ ⌜int.Z tid ≤ int.Z tidlast ∨ int.Z tidown = 0⌝ ∗
     "%Hret" ∷ ⌜spec_lookup vers tid = to_dbval found val⌝.
 
-Definition per_key_cmt_inv_def key tmods tid m past future γ : iProp Σ :=
-  per_key_inv_def γ key tmods tid m past ∗ cmt_inv_def γ tmods future.
-
 Lemma tuple_read_safe (tid : u64) ts key tmods m past future tuple val found γ :
   let tidN := (int.nat tid) in 
   head_read future tidN key ->
   ([∗ set] k ∈ keys_all, per_key_inv_def γ k tmods ts m past) -∗
-  cmt_inv_def γ tmods future -∗
+  cmt_inv_def γ tmods future ts -∗
   tuple_read tuple tid key val found γ ==∗
   ([∗ set] k ∈ keys_all, per_key_inv_def γ k tmods ts m (past ++ [EvRead tidN key])) ∗
-  cmt_inv_def γ tmods future ∗
+  cmt_inv_def γ tmods future ts ∗
   own_tuple tuple key γ ∗
   ptuple_ptsto γ key (to_dbval found val) tidN.
 Admitted.
